Zag.lean
@@ -2,6 +2,12 @@
 -- Import modules here that should be built as part of the library.
 import Zag.Data
 import Zag.Theory
+import Zag.Machine
+import Zag.Weakening
+import Zag.Machine
+import Zag.Weakening
 import Zag.EvalState
+import Zag.Loop
+import Zag.Loop
 import Zag.Syntax
 import Zag.Meta
